document.thy
@@ -1,0 +1,10 @@
+theory document
+  imports Lsharp
+begin
+
+text \<open> for example for \<open>rule2\<close> we prove @{term "norm1 (S,F,T) = norm1 (S',F',T')"}, 
+@{term "norm2 (S,F,T) < norm2 (S',F',T')"} and @{term "norm3 (S,F,T) \<le> norm3 (S',F',T')"} resulting in 
+@{term "norm (S,F,T)<norm (S',F',T')"}\<close>
+
+
+end
