ROOT
@@ -1,0 +1,14 @@
+session "Fsharp-isabelle" = HOL + options [document = pdf, document_output = "output", quick_and_dirty=true]
+ sessions
+  "HOL-Library" 
+ 
+  
+theories 
+  MealyMachine
+   Lsharp
+ theories 
+ document
+  
+
+document_files
+    "root.tex"
